LiveVerif/src/LiveVerif/LiveVerifLib.v
@@ -24,6 +24,7 @@ Require Export bedrock2.HeapletwiseHyps.
 Require Export bedrock2.HeapletwiseAutoSplitMerge.
 Require Export bedrock2.bottom_up_simpl.
 Require Export bedrock2.TacticError.
+Require Export bedrock2.SuppressibleWarnings.
 Require Export bedrock2.SepLib.
 Require Export bedrock2.PurifySep.
 Require Export bedrock2.PurifyHeapletwise.
