bedrock2/src/bedrock2/SuppressibleWarnings.v
@@ -1,0 +1,53 @@
+Declare Scope message_scope.
+Definition message_scope_marker{T: Type}(msg: T) := msg.
+Arguments message_scope_marker {T} msg%message_scope.
+
+(* Call this tactic to obtain a pattern-matchable representation of the warning *)
+Ltac unexplain := unfold message_scope_marker in *.
+
+Notation "x" := (message_scope_marker x) (at level 100, only printing).
+
+(* Convention: All warnings whose type can be proved by `eauto with suppressed_warnings`
+   will be suppressed.
+   This has the nice side effect that warnings which already appear in the context
+   will not be posed again. *)
+Create HintDb suppressed_warnings.
+
+Ltac pose_warning w :=
+  let t := type of w in
+  tryif (let __ := constr:(ltac:(eauto with suppressed_warnings): t) in idtac)
+  then idtac (*suppressed*)
+  else let name := fresh "Warning" in pose proof (w : message_scope_marker t) as name.
+
+Module Examples.
+  Inductive no_frobnicator_found(terms: list nat)(T: Type)(x: T): Set :=
+    mk_sample_no_frobnicator_found.
+
+  Notation "'At' 'least' 'one' 'of' 'the' 'terms' t1 , .. , tn 'should' 'have' 'a' 'frobnicator' 'that' 'works' 'under' x 'of' 'type' T" :=
+  (no_frobnicator_found (cons t1 .. (cons tn nil) ..) T x)
+  (at level 1, t1 at level 0, tn at level 0, only printing)
+  : message_scope.
+
+  Ltac sample_tac b :=
+    lazymatch goal with
+    | |- ?n = _ =>
+        pose_warning (mk_sample_no_frobnicator_found
+                        (cons (1 + 1) (cons (4 - 2) nil)) (nat * bool) (n, b))
+    end.
+
+  Goal exists (n: nat), n = n.
+    eexists.
+    sample_tac true. (* displays a warning *)
+    sample_tac true. (* doesn't duplicate the same warning *)
+    unexplain. (* displays the warning in a pattern-matchable way *)
+
+    (* Example: Let's say it's ok if a true-pair frobnicator can't be found: *)
+    Local Hint Extern 1 (no_frobnicator_found _ (_ * _) (_, true)) =>
+      constructor : suppressed_warnings.
+
+    clear Warning.
+
+    sample_tac true. (* no warning any more *)
+    sample_tac false. (* but this one is still shown *)
+  Abort.
+End Examples.
